x86/proofs/p384_montjmixadd.ml
@@ -4549,61 +4549,114 @@ let p384_montjmixadd_mc = define_assert_from_elf
   0x49; 0x83; 0xdb; 0x00;  (* SBB (% r11) (Imm8 (word 0)) *)
   0x4c; 0x89; 0x9c; 0x24; 0xe8; 0x00; 0x00; 0x00;
                            (* MOV (Memop Quadword (%% (rsp,232))) (% r11) *)
-  0x48; 0x8b; 0x04; 0x24;  (* MOV (% rax) (Memop Quadword (%% (rsp,0))) *)
-  0x48; 0x89; 0x07;        (* MOV (Memop Quadword (%% (rdi,0))) (% rax) *)
-  0x48; 0x8b; 0x44; 0x24; 0x08;
-                           (* MOV (% rax) (Memop Quadword (%% (rsp,8))) *)
-  0x48; 0x89; 0x47; 0x08;  (* MOV (Memop Quadword (%% (rdi,8))) (% rax) *)
-  0x48; 0x8b; 0x44; 0x24; 0x10;
-                           (* MOV (% rax) (Memop Quadword (%% (rsp,16))) *)
-  0x48; 0x89; 0x47; 0x10;  (* MOV (Memop Quadword (%% (rdi,16))) (% rax) *)
-  0x48; 0x8b; 0x44; 0x24; 0x18;
-                           (* MOV (% rax) (Memop Quadword (%% (rsp,24))) *)
-  0x48; 0x89; 0x47; 0x18;  (* MOV (Memop Quadword (%% (rdi,24))) (% rax) *)
-  0x48; 0x8b; 0x44; 0x24; 0x20;
-                           (* MOV (% rax) (Memop Quadword (%% (rsp,32))) *)
-  0x48; 0x89; 0x47; 0x20;  (* MOV (Memop Quadword (%% (rdi,32))) (% rax) *)
-  0x48; 0x8b; 0x44; 0x24; 0x28;
-                           (* MOV (% rax) (Memop Quadword (%% (rsp,40))) *)
-  0x48; 0x89; 0x47; 0x28;  (* MOV (Memop Quadword (%% (rdi,40))) (% rax) *)
-  0x48; 0x8b; 0x84; 0x24; 0xc0; 0x00; 0x00; 0x00;
-                           (* MOV (% rax) (Memop Quadword (%% (rsp,192))) *)
-  0x48; 0x89; 0x47; 0x30;  (* MOV (Memop Quadword (%% (rdi,48))) (% rax) *)
-  0x48; 0x8b; 0x84; 0x24; 0xc8; 0x00; 0x00; 0x00;
-                           (* MOV (% rax) (Memop Quadword (%% (rsp,200))) *)
-  0x48; 0x89; 0x47; 0x38;  (* MOV (Memop Quadword (%% (rdi,56))) (% rax) *)
-  0x48; 0x8b; 0x84; 0x24; 0xd0; 0x00; 0x00; 0x00;
-                           (* MOV (% rax) (Memop Quadword (%% (rsp,208))) *)
-  0x48; 0x89; 0x47; 0x40;  (* MOV (Memop Quadword (%% (rdi,64))) (% rax) *)
-  0x48; 0x8b; 0x84; 0x24; 0xd8; 0x00; 0x00; 0x00;
-                           (* MOV (% rax) (Memop Quadword (%% (rsp,216))) *)
-  0x48; 0x89; 0x47; 0x48;  (* MOV (Memop Quadword (%% (rdi,72))) (% rax) *)
-  0x48; 0x8b; 0x84; 0x24; 0xe0; 0x00; 0x00; 0x00;
-                           (* MOV (% rax) (Memop Quadword (%% (rsp,224))) *)
-  0x48; 0x89; 0x47; 0x50;  (* MOV (Memop Quadword (%% (rdi,80))) (% rax) *)
-  0x48; 0x8b; 0x84; 0x24; 0xe8; 0x00; 0x00; 0x00;
-                           (* MOV (% rax) (Memop Quadword (%% (rsp,232))) *)
-  0x48; 0x89; 0x47; 0x58;  (* MOV (Memop Quadword (%% (rdi,88))) (% rax) *)
-  0x48; 0x8b; 0x84; 0x24; 0xf0; 0x00; 0x00; 0x00;
-                           (* MOV (% rax) (Memop Quadword (%% (rsp,240))) *)
-  0x48; 0x89; 0x47; 0x60;  (* MOV (Memop Quadword (%% (rdi,96))) (% rax) *)
-  0x48; 0x8b; 0x84; 0x24; 0xf8; 0x00; 0x00; 0x00;
-                           (* MOV (% rax) (Memop Quadword (%% (rsp,248))) *)
-  0x48; 0x89; 0x47; 0x68;  (* MOV (Memop Quadword (%% (rdi,104))) (% rax) *)
-  0x48; 0x8b; 0x84; 0x24; 0x00; 0x01; 0x00; 0x00;
-                           (* MOV (% rax) (Memop Quadword (%% (rsp,256))) *)
-  0x48; 0x89; 0x47; 0x70;  (* MOV (Memop Quadword (%% (rdi,112))) (% rax) *)
-  0x48; 0x8b; 0x84; 0x24; 0x08; 0x01; 0x00; 0x00;
-                           (* MOV (% rax) (Memop Quadword (%% (rsp,264))) *)
-  0x48; 0x89; 0x47; 0x78;  (* MOV (Memop Quadword (%% (rdi,120))) (% rax) *)
-  0x48; 0x8b; 0x84; 0x24; 0x10; 0x01; 0x00; 0x00;
-                           (* MOV (% rax) (Memop Quadword (%% (rsp,272))) *)
-  0x48; 0x89; 0x87; 0x80; 0x00; 0x00; 0x00;
-                           (* MOV (Memop Quadword (%% (rdi,128))) (% rax) *)
-  0x48; 0x8b; 0x84; 0x24; 0x18; 0x01; 0x00; 0x00;
-                           (* MOV (% rax) (Memop Quadword (%% (rsp,280))) *)
-  0x48; 0x89; 0x87; 0x88; 0x00; 0x00; 0x00;
-                           (* MOV (Memop Quadword (%% (rdi,136))) (% rax) *)
+  0x48; 0x8b; 0xb4; 0x24; 0x20; 0x01; 0x00; 0x00;
+                           (* MOV (% rsi) (Memop Quadword (%% (rsp,288))) *)
+  0x48; 0x8b; 0x46; 0x60;  (* MOV (% rax) (Memop Quadword (%% (rsi,96))) *)
+  0x48; 0x8b; 0x56; 0x68;  (* MOV (% rdx) (Memop Quadword (%% (rsi,104))) *)
+  0x48; 0x0b; 0x46; 0x70;  (* OR (% rax) (Memop Quadword (%% (rsi,112))) *)
+  0x48; 0x0b; 0x56; 0x78;  (* OR (% rdx) (Memop Quadword (%% (rsi,120))) *)
+  0x48; 0x0b; 0x86; 0x80; 0x00; 0x00; 0x00;
+                           (* OR (% rax) (Memop Quadword (%% (rsi,128))) *)
+  0x48; 0x0b; 0x96; 0x88; 0x00; 0x00; 0x00;
+                           (* OR (% rdx) (Memop Quadword (%% (rsi,136))) *)
+  0x48; 0x09; 0xd0;        (* OR (% rax) (% rdx) *)
+  0x48; 0x8b; 0x8c; 0x24; 0x28; 0x01; 0x00; 0x00;
+                           (* MOV (% rcx) (Memop Quadword (%% (rsp,296))) *)
+  0x48; 0x8b; 0x01;        (* MOV (% rax) (Memop Quadword (%% (rcx,0))) *)
+  0x4c; 0x8b; 0x04; 0x24;  (* MOV (% r8) (Memop Quadword (%% (rsp,0))) *)
+  0x4c; 0x0f; 0x44; 0xc0;  (* CMOVE (% r8) (% rax) *)
+  0x48; 0x8b; 0x41; 0x08;  (* MOV (% rax) (Memop Quadword (%% (rcx,8))) *)
+  0x4c; 0x8b; 0x4c; 0x24; 0x08;
+                           (* MOV (% r9) (Memop Quadword (%% (rsp,8))) *)
+  0x4c; 0x0f; 0x44; 0xc8;  (* CMOVE (% r9) (% rax) *)
+  0x48; 0x8b; 0x41; 0x10;  (* MOV (% rax) (Memop Quadword (%% (rcx,16))) *)
+  0x4c; 0x8b; 0x54; 0x24; 0x10;
+                           (* MOV (% r10) (Memop Quadword (%% (rsp,16))) *)
+  0x4c; 0x0f; 0x44; 0xd0;  (* CMOVE (% r10) (% rax) *)
+  0x48; 0x8b; 0x41; 0x18;  (* MOV (% rax) (Memop Quadword (%% (rcx,24))) *)
+  0x4c; 0x8b; 0x5c; 0x24; 0x18;
+                           (* MOV (% r11) (Memop Quadword (%% (rsp,24))) *)
+  0x4c; 0x0f; 0x44; 0xd8;  (* CMOVE (% r11) (% rax) *)
+  0x48; 0x8b; 0x41; 0x20;  (* MOV (% rax) (Memop Quadword (%% (rcx,32))) *)
+  0x48; 0x8b; 0x5c; 0x24; 0x20;
+                           (* MOV (% rbx) (Memop Quadword (%% (rsp,32))) *)
+  0x48; 0x0f; 0x44; 0xd8;  (* CMOVE (% rbx) (% rax) *)
+  0x48; 0x8b; 0x41; 0x28;  (* MOV (% rax) (Memop Quadword (%% (rcx,40))) *)
+  0x48; 0x8b; 0x6c; 0x24; 0x28;
+                           (* MOV (% rbp) (Memop Quadword (%% (rsp,40))) *)
+  0x48; 0x0f; 0x44; 0xe8;  (* CMOVE (% rbp) (% rax) *)
+  0x48; 0x8b; 0x41; 0x30;  (* MOV (% rax) (Memop Quadword (%% (rcx,48))) *)
+  0x4c; 0x8b; 0xa4; 0x24; 0xc0; 0x00; 0x00; 0x00;
+                           (* MOV (% r12) (Memop Quadword (%% (rsp,192))) *)
+  0x4c; 0x0f; 0x44; 0xe0;  (* CMOVE (% r12) (% rax) *)
+  0x48; 0x8b; 0x41; 0x38;  (* MOV (% rax) (Memop Quadword (%% (rcx,56))) *)
+  0x4c; 0x8b; 0xac; 0x24; 0xc8; 0x00; 0x00; 0x00;
+                           (* MOV (% r13) (Memop Quadword (%% (rsp,200))) *)
+  0x4c; 0x0f; 0x44; 0xe8;  (* CMOVE (% r13) (% rax) *)
+  0x48; 0x8b; 0x41; 0x40;  (* MOV (% rax) (Memop Quadword (%% (rcx,64))) *)
+  0x4c; 0x8b; 0xb4; 0x24; 0xd0; 0x00; 0x00; 0x00;
+                           (* MOV (% r14) (Memop Quadword (%% (rsp,208))) *)
+  0x4c; 0x0f; 0x44; 0xf0;  (* CMOVE (% r14) (% rax) *)
+  0x48; 0x8b; 0x41; 0x48;  (* MOV (% rax) (Memop Quadword (%% (rcx,72))) *)
+  0x4c; 0x8b; 0xbc; 0x24; 0xd8; 0x00; 0x00; 0x00;
+                           (* MOV (% r15) (Memop Quadword (%% (rsp,216))) *)
+  0x4c; 0x0f; 0x44; 0xf8;  (* CMOVE (% r15) (% rax) *)
+  0x48; 0x8b; 0x41; 0x50;  (* MOV (% rax) (Memop Quadword (%% (rcx,80))) *)
+  0x48; 0x8b; 0x94; 0x24; 0xe0; 0x00; 0x00; 0x00;
+                           (* MOV (% rdx) (Memop Quadword (%% (rsp,224))) *)
+  0x48; 0x0f; 0x44; 0xd0;  (* CMOVE (% rdx) (% rax) *)
+  0x48; 0x8b; 0x41; 0x58;  (* MOV (% rax) (Memop Quadword (%% (rcx,88))) *)
+  0x48; 0x8b; 0x8c; 0x24; 0xe8; 0x00; 0x00; 0x00;
+                           (* MOV (% rcx) (Memop Quadword (%% (rsp,232))) *)
+  0x48; 0x0f; 0x44; 0xc8;  (* CMOVE (% rcx) (% rax) *)
+  0x48; 0x8b; 0xbc; 0x24; 0x30; 0x01; 0x00; 0x00;
+                           (* MOV (% rdi) (Memop Quadword (%% (rsp,304))) *)
+  0x4c; 0x89; 0x07;        (* MOV (Memop Quadword (%% (rdi,0))) (% r8) *)
+  0x4c; 0x89; 0x4f; 0x08;  (* MOV (Memop Quadword (%% (rdi,8))) (% r9) *)
+  0x4c; 0x89; 0x57; 0x10;  (* MOV (Memop Quadword (%% (rdi,16))) (% r10) *)
+  0x4c; 0x89; 0x5f; 0x18;  (* MOV (Memop Quadword (%% (rdi,24))) (% r11) *)
+  0x48; 0x89; 0x5f; 0x20;  (* MOV (Memop Quadword (%% (rdi,32))) (% rbx) *)
+  0x48; 0x89; 0x6f; 0x28;  (* MOV (Memop Quadword (%% (rdi,40))) (% rbp) *)
+  0x4c; 0x89; 0x67; 0x30;  (* MOV (Memop Quadword (%% (rdi,48))) (% r12) *)
+  0x4c; 0x89; 0x6f; 0x38;  (* MOV (Memop Quadword (%% (rdi,56))) (% r13) *)
+  0x4c; 0x89; 0x77; 0x40;  (* MOV (Memop Quadword (%% (rdi,64))) (% r14) *)
+  0x4c; 0x89; 0x7f; 0x48;  (* MOV (Memop Quadword (%% (rdi,72))) (% r15) *)
+  0x48; 0x89; 0x57; 0x50;  (* MOV (Memop Quadword (%% (rdi,80))) (% rdx) *)
+  0x48; 0x89; 0x4f; 0x58;  (* MOV (Memop Quadword (%% (rdi,88))) (% rcx) *)
+  0x4c; 0x8b; 0x84; 0x24; 0xf0; 0x00; 0x00; 0x00;
+                           (* MOV (% r8) (Memop Quadword (%% (rsp,240))) *)
+  0x4c; 0x8b; 0x8c; 0x24; 0xf8; 0x00; 0x00; 0x00;
+                           (* MOV (% r9) (Memop Quadword (%% (rsp,248))) *)
+  0x4c; 0x8b; 0x94; 0x24; 0x00; 0x01; 0x00; 0x00;
+                           (* MOV (% r10) (Memop Quadword (%% (rsp,256))) *)
+  0x4c; 0x8b; 0x9c; 0x24; 0x08; 0x01; 0x00; 0x00;
+                           (* MOV (% r11) (Memop Quadword (%% (rsp,264))) *)
+  0x48; 0x8b; 0x9c; 0x24; 0x10; 0x01; 0x00; 0x00;
+                           (* MOV (% rbx) (Memop Quadword (%% (rsp,272))) *)
+  0x48; 0x8b; 0xac; 0x24; 0x18; 0x01; 0x00; 0x00;
+                           (* MOV (% rbp) (Memop Quadword (%% (rsp,280))) *)
+  0x48; 0xb8; 0x01; 0x00; 0x00; 0x00; 0xff; 0xff; 0xff; 0xff;
+                           (* MOV (% rax) (Imm64 (word 18446744069414584321)) *)
+  0x4c; 0x0f; 0x44; 0xc0;  (* CMOVE (% r8) (% rax) *)
+  0xb8; 0xff; 0xff; 0xff; 0xff;
+                           (* MOV (% eax) (Imm32 (word 4294967295)) *)
+  0x4c; 0x0f; 0x44; 0xc8;  (* CMOVE (% r9) (% rax) *)
+  0x48; 0xc7; 0xc0; 0x01; 0x00; 0x00; 0x00;
+                           (* MOV (% rax) (Imm32 (word 1)) *)
+  0x4c; 0x0f; 0x44; 0xd0;  (* CMOVE (% r10) (% rax) *)
+  0xb8; 0x00; 0x00; 0x00; 0x00;
+                           (* MOV (% eax) (Imm32 (word 0)) *)
+  0x4c; 0x0f; 0x44; 0xd8;  (* CMOVE (% r11) (% rax) *)
+  0x48; 0x0f; 0x44; 0xd8;  (* CMOVE (% rbx) (% rax) *)
+  0x48; 0x0f; 0x44; 0xe8;  (* CMOVE (% rbp) (% rax) *)
+  0x4c; 0x89; 0x47; 0x60;  (* MOV (Memop Quadword (%% (rdi,96))) (% r8) *)
+  0x4c; 0x89; 0x4f; 0x68;  (* MOV (Memop Quadword (%% (rdi,104))) (% r9) *)
+  0x4c; 0x89; 0x57; 0x70;  (* MOV (Memop Quadword (%% (rdi,112))) (% r10) *)
+  0x4c; 0x89; 0x5f; 0x78;  (* MOV (Memop Quadword (%% (rdi,120))) (% r11) *)
+  0x48; 0x89; 0x9f; 0x80; 0x00; 0x00; 0x00;
+                           (* MOV (Memop Quadword (%% (rdi,128))) (% rbx) *)
+  0x48; 0x89; 0xaf; 0x88; 0x00; 0x00; 0x00;
+                           (* MOV (Memop Quadword (%% (rdi,136))) (% rbp) *)
   0x48; 0x81; 0xc4; 0x38; 0x01; 0x00; 0x00;
                            (* ADD (% rsp) (Imm32 (word 312)) *)
   0x41; 0x5f;              (* POP (% r15) *)
@@ -4620,72 +4673,6 @@ let P384_MONTJMIXADD_EXEC = X86_MK_CORE_EXEC_RULE p384_montjmixadd_mc;;
 (* ------------------------------------------------------------------------- *)
 (* Common supporting definitions and lemmas for component proofs.            *)
 (* ------------------------------------------------------------------------- *)
-
-let p_384 = new_definition `p_384 = 39402006196394479212279040100143613805079739270465446667948293404245721771496870329047266088258938001861606973112319`;;
-
-let nistp384 = define
- `nistp384 =
-    (integer_mod_ring p_384,
-     ring_neg (integer_mod_ring p_384) (&3),
-     &b_384:int)`;;
-
-let nistp384_encode = new_definition
-  `nistp384_encode = montgomery_encode(384,p_384)`;;
-
-let swlemma = WORD_RULE
-  `word_add (word_shl x 32) x:int64 = word(4294967297 * val x)`;;
-
-let mmlemma = prove
- (`!h (l:int64) (x:int64).
-        &2 pow 64 * &h + &(val(l:int64)):real =
-        &(val(word(4294967297 * val x):int64)) * &18446744069414584321
-        ==> &2 pow 64 * &h + &(val(x:int64)):real =
-            &(val(word(4294967297 * val x):int64)) * &18446744069414584321`,
-  REPEAT GEN_TAC THEN REWRITE_TAC[REAL_OF_NUM_CLAUSES] THEN
-  REPEAT STRIP_TAC THEN FIRST_ASSUM(SUBST1_TAC o SYM) THEN
-  AP_TERM_TAC THEN AP_TERM_TAC THEN
-  REWRITE_TAC[GSYM VAL_CONG; DIMINDEX_64] THEN FIRST_X_ASSUM(MATCH_MP_TAC o
-   MATCH_MP (NUMBER_RULE
-    `p * h + l:num = y ==> (y == x) (mod p) ==> (x == l) (mod p)`)) THEN
-  REWRITE_TAC[CONG; VAL_WORD; DIMINDEX_64] THEN CONV_TAC MOD_DOWN_CONV THEN
-  REWRITE_TAC[GSYM CONG] THEN MATCH_MP_TAC(NUMBER_RULE
-   `(a * b == 1) (mod p) ==> ((a * x) * b == x) (mod p)`) THEN
-  REWRITE_TAC[CONG] THEN CONV_TAC NUM_REDUCE_CONV);;
-
-let nintlemma = prove
- (`&(num_of_int(x rem &p_384)) = x rem &p_384`,
-  MATCH_MP_TAC INT_OF_NUM_OF_INT THEN MATCH_MP_TAC INT_REM_POS THEN
-  REWRITE_TAC[INT_OF_NUM_EQ; p_384] THEN CONV_TAC NUM_REDUCE_CONV);;
-
-let unilemma0 = prove
- (`x = a MOD p_384 ==> x < p_384 /\ &x = &a rem &p_384`,
-  REWRITE_TAC[INT_OF_NUM_REM; p_384] THEN ARITH_TAC);;
-
-let unilemma1 = prove
- (`&x = a rem &p_384 ==> x < p_384 /\ &x = a rem &p_384`,
-  SIMP_TAC[GSYM INT_OF_NUM_LT; INT_LT_REM_EQ; p_384] THEN INT_ARITH_TAC);;
-
-let unilemma2 = prove
- (`X = num_of_int(x rem &p_384) ==> X < p_384 /\ &X = x rem &p_384`,
-  DISCH_THEN SUBST1_TAC THEN
-  REWRITE_TAC[GSYM INT_OF_NUM_LT; nintlemma; INT_LT_REM_EQ] THEN
-  REWRITE_TAC[INT_OF_NUM_LT; p_384] THEN CONV_TAC NUM_REDUCE_CONV);;
-
-let lemont = prove
- (`(&i * x * y) rem &p_384 = (&i * x rem &p_384 * y rem &p_384) rem &p_384`,
-  CONV_TAC INT_REM_DOWN_CONV THEN REWRITE_TAC[]);;
-
-let pumont = prove
- (`(&(inverse_mod p_384 (2 EXP 384)) *
-    (&2 pow 384 * x) rem &p_384 * (&2 pow 384 * y) rem &p_384) rem &p_384 =
-   (&2 pow 384 * x * y) rem &p_384`,
-  CONV_TAC INT_REM_DOWN_CONV THEN REWRITE_TAC[INT_REM_EQ] THEN
-  MATCH_MP_TAC(INTEGER_RULE
-   `(i * t:int == &1) (mod p)
-    ==> (i * (t * x) * (t * y) == t * x * y) (mod p)`) THEN
-  REWRITE_TAC[GSYM num_congruent; INT_OF_NUM_CLAUSES] THEN
-  REWRITE_TAC[INVERSE_MOD_LMUL_EQ; COPRIME_REXP; COPRIME_2; p_384] THEN
-  CONV_TAC NUM_REDUCE_CONV);;
 
 let lvs =
  ["x_1",[`RSI`;`0`];
@@ -4713,6 +4700,26 @@ let lvs =
 
 let DESUM_RULE' = cache DESUM_RULE and DECARRY_RULE' = cache DECARRY_RULE;;
 
+let swlemma = WORD_RULE
+  `word_add (word_shl x 32) x:int64 = word(4294967297 * val x)`;;
+
+let mmlemma = prove
+ (`!h (l:int64) (x:int64).
+        &2 pow 64 * &h + &(val(l:int64)):real =
+        &(val(word(4294967297 * val x):int64)) * &18446744069414584321
+        ==> &2 pow 64 * &h + &(val(x:int64)):real =
+            &(val(word(4294967297 * val x):int64)) * &18446744069414584321`,
+  REPEAT GEN_TAC THEN REWRITE_TAC[REAL_OF_NUM_CLAUSES] THEN
+  REPEAT STRIP_TAC THEN FIRST_ASSUM(SUBST1_TAC o SYM) THEN
+  AP_TERM_TAC THEN AP_TERM_TAC THEN
+  REWRITE_TAC[GSYM VAL_CONG; DIMINDEX_64] THEN FIRST_X_ASSUM(MATCH_MP_TAC o
+   MATCH_MP (NUMBER_RULE
+    `p * h + l:num = y ==> (y == x) (mod p) ==> (x == l) (mod p)`)) THEN
+  REWRITE_TAC[CONG; VAL_WORD; DIMINDEX_64] THEN CONV_TAC MOD_DOWN_CONV THEN
+  REWRITE_TAC[GSYM CONG] THEN MATCH_MP_TAC(NUMBER_RULE
+   `(a * b == 1) (mod p) ==> ((a * x) * b == x) (mod p)`) THEN
+  REWRITE_TAC[CONG] THEN CONV_TAC NUM_REDUCE_CONV);;
+
 (* ------------------------------------------------------------------------- *)
 (* Instances of montsqr.                                                     *)
 (* ------------------------------------------------------------------------- *)
@@ -4722,7 +4729,7 @@ let LOCAL_MONTSQR_P384_TAC =
   `!(t:x86state) pcin pcout p3 n3 p1 n1.
     !a. read(memory :> bytes(word_add (read p1 t) (word n1),8 * 6)) t = a
     ==>
-    nonoverlapping (word pc,0x3b3a) (word_add (read p3 t) (word n3),48)
+    nonoverlapping (word pc,0x3c05) (word_add (read p3 t) (word n3),48)
     ==> ensures x86
          (\s. bytes_loaded s (word pc) (BUTLAST p384_montjmixadd_mc) /\
               read RIP s = pcin /\
@@ -4861,7 +4868,7 @@ let LOCAL_MONTMUL_P384_TAC =
     ==>
     !b. read(memory :> bytes(word_add (read p2 t) (word n2),8 * 6)) t = b
     ==>
-    nonoverlapping (word pc,0x3b3a) (word_add (read p3 t) (word n3),48)
+    nonoverlapping (word pc,0x3c05) (word_add (read p3 t) (word n3),48)
     ==> ensures x86
          (\s. bytes_loaded s (word pc) (BUTLAST p384_montjmixadd_mc) /\
               read RIP s = pcin /\
@@ -5013,7 +5020,7 @@ let LOCAL_SUB_P384_TAC =
     ==>
     !n. read(memory :> bytes(word_add (read p2 t) (word n2),8 * 6)) t = n
     ==>
-    nonoverlapping (word pc,0x3b3a) (word_add (read p3 t) (word n3),48)
+    nonoverlapping (word pc,0x3c05) (word_add (read p3 t) (word n3),48)
     ==> ensures x86
          (\s. bytes_loaded s (word pc) (BUTLAST p384_montjmixadd_mc) /\
               read RIP s = pcin /\
@@ -5103,7 +5110,7 @@ let LOCAL_AMONTSQR_P384_TAC =
   `!(t:x86state) pcin pcout p3 n3 p1 n1.
     !a. read(memory :> bytes(word_add (read p1 t) (word n1),8 * 6)) t = a
     ==>
-    nonoverlapping (word pc,0x3b3a) (word_add (read p3 t) (word n3),48)
+    nonoverlapping (word pc,0x3c05) (word_add (read p3 t) (word n3),48)
     ==> ensures x86
          (\s. bytes_loaded s (word pc) (BUTLAST p384_montjmixadd_mc) /\
               read RIP s = pcin /\
@@ -5213,11 +5220,124 @@ let LOCAL_AMONTSQR_P384_TAC =
 (* Overall point operation proof.                                            *)
 (* ------------------------------------------------------------------------- *)
 
+let unilemma0 = prove
+ (`x = a MOD p_384 ==> x < p_384 /\ &x = &a rem &p_384`,
+  REWRITE_TAC[INT_OF_NUM_REM; p_384] THEN ARITH_TAC);;
+
+let unilemma1 = prove
+ (`&x = a rem &p_384 ==> x < p_384 /\ &x = a rem &p_384`,
+  SIMP_TAC[GSYM INT_OF_NUM_LT; INT_LT_REM_EQ; p_384] THEN INT_ARITH_TAC);;
+
+let lemont = prove
+ (`(&i * x * y) rem &p_384 = (&i * x rem &p_384 * y rem &p_384) rem &p_384`,
+  CONV_TAC INT_REM_DOWN_CONV THEN REWRITE_TAC[]);;
+
+let demont = prove
+ (`(&(NUMERAL n) * &x) rem &p_384 = (&(NUMERAL n) * &x rem &p_384) rem &p_384`,
+  CONV_TAC INT_REM_DOWN_CONV THEN REWRITE_TAC[]);;
+
+let pumont = prove
+ (`(&(inverse_mod p_384 (2 EXP 384)) *
+    (&2 pow 384 * x) rem &p_384 * (&2 pow 384 * y) rem &p_384) rem &p_384 =
+   (&2 pow 384 * x * y) rem &p_384`,
+  CONV_TAC INT_REM_DOWN_CONV THEN REWRITE_TAC[INT_REM_EQ] THEN
+  MATCH_MP_TAC(INTEGER_RULE
+   `(i * t:int == &1) (mod p)
+    ==> (i * (t * x) * (t * y) == t * x * y) (mod p)`) THEN
+  REWRITE_TAC[GSYM num_congruent; INT_OF_NUM_CLAUSES] THEN
+  REWRITE_TAC[INVERSE_MOD_LMUL_EQ; COPRIME_REXP; COPRIME_2; p_384] THEN
+  CONV_TAC NUM_REDUCE_CONV);;
+
+let dismont = prove
+ (`((&2 pow 384 * x) rem &p_384 + (&2 pow 384 * y) rem &p_384) rem &p_384 =
+   (&2 pow 384 * (x + y)) rem &p_384 /\
+   ((&2 pow 384 * x) rem &p_384 - (&2 pow 384 * y) rem &p_384) rem &p_384 =
+   (&2 pow 384 * (x - y)) rem &p_384 /\
+   (&(NUMERAL n) * (&2 pow 384 * x) rem &p_384) rem &p_384 =
+   (&2 pow 384 * (&(NUMERAL n) * x)) rem &p_384`,
+  REPEAT CONJ_TAC THEN CONV_TAC INT_REM_DOWN_CONV THEN
+  AP_THM_TAC THEN AP_TERM_TAC THEN INT_ARITH_TAC);;
+
+let unmont = prove
+ (`(&(inverse_mod p_384 (2 EXP 384)) * (&2 pow 384 * x) rem &p_384) rem &p_384 =
+   x rem &p_384`,
+  CONV_TAC INT_REM_DOWN_CONV THEN REWRITE_TAC[INT_REM_EQ] THEN
+  MATCH_MP_TAC(INTEGER_RULE
+   `(i * e:int == &1) (mod p) ==> (i * e * x == x) (mod p)`) THEN
+  REWRITE_TAC[INT_OF_NUM_CLAUSES; GSYM num_congruent; INVERSE_MOD_LMUL_EQ] THEN
+  REWRITE_TAC[COPRIME_REXP; COPRIME_2; p_384] THEN CONV_TAC NUM_REDUCE_CONV);;
+
+let unreplemma = prove
+ (`!x. x < p_384
+         ==> x =
+             (2 EXP 384 * (inverse_mod p_384 (2 EXP 384) * x) MOD p_384) MOD
+             p_384`,
+  REPEAT STRIP_TAC THEN CONV_TAC SYM_CONV THEN
+  ASM_REWRITE_TAC[MOD_UNIQUE] THEN
+  REWRITE_TAC[CONG] THEN CONV_TAC MOD_DOWN_CONV THEN
+  REWRITE_TAC[GSYM CONG] THEN MATCH_MP_TAC(NUMBER_RULE
+   `(i * e == 1) (mod p) ==> (i * e * x == x) (mod p)`) THEN
+  REWRITE_TAC[INVERSE_MOD_RMUL_EQ] THEN
+  REWRITE_TAC[COPRIME_REXP; COPRIME_2; p_384] THEN CONV_TAC NUM_REDUCE_CONV);;
+
+let weierstrass_of_affine_p384 = prove
+ (`weierstrass_of_jacobian (integer_mod_ring p_384)
+                           (x rem &p_384,y rem &p_384,&1 rem &p_384) =
+   SOME(x rem &p_384,y rem &p_384)`,
+  MP_TAC(ISPEC `integer_mod_ring p_384` RING_INV_1) THEN
+  REWRITE_TAC[weierstrass_of_jacobian; ring_div; INTEGER_MOD_RING_CLAUSES] THEN
+  REWRITE_TAC[p_384] THEN CONV_TAC INT_REDUCE_CONV THEN
+  SIMP_TAC[GSYM p_384; option_INJ; PAIR_EQ; INT_MUL_RID; INT_REM_REM]);;
+
+let weierstrass_of_jacobian_p384_add = prove
+ (`!P1 P2 x1 y1 z1 x2 y2 z2 x3 y3 z3.
+        ~(weierstrass_of_jacobian (integer_mod_ring p_384)
+           (x1 rem &p_384,y1 rem &p_384,z1 rem &p_384) =
+          weierstrass_of_jacobian (integer_mod_ring p_384)
+           (x2 rem &p_384,y2 rem &p_384,z2 rem &p_384)) /\
+        jacobian_add_unexceptional nistp384
+         (x1 rem &p_384,y1 rem &p_384,z1 rem &p_384)
+         (x2 rem &p_384,y2 rem &p_384,z2 rem &p_384) =
+        (x3 rem &p_384,y3 rem &p_384,z3 rem &p_384)
+        ==> weierstrass_of_jacobian (integer_mod_ring p_384)
+                (x1 rem &p_384,y1 rem &p_384,z1 rem &p_384) = P1 /\
+            weierstrass_of_jacobian (integer_mod_ring p_384)
+                (x2 rem &p_384,y2 rem &p_384,z2 rem &p_384) = P2
+            ==> weierstrass_of_jacobian (integer_mod_ring p_384)
+                  (x3 rem &p_384,y3 rem &p_384,z3 rem &p_384) =
+                group_mul p384_group P1 P2`,
+  REPEAT GEN_TAC THEN
+  DISCH_THEN(CONJUNCTS_THEN2 ASSUME_TAC (SUBST1_TAC o SYM)) THEN
+  DISCH_THEN(CONJUNCTS_THEN(SUBST1_TAC o SYM)) THEN
+  REWRITE_TAC[nistp384; P384_GROUP] THEN
+  MATCH_MP_TAC WEIERSTRASS_OF_JACOBIAN_ADD_UNEXCEPTIONAL THEN
+  REWRITE_TAC[CONJ_ASSOC] THEN CONJ_TAC THENL
+   [ALL_TAC;
+    W(MP_TAC o PART_MATCH (rand o rand) WEIERSTRASS_OF_JACOBIAN_EQ o
+      rand o snd) THEN
+    ASM_REWRITE_TAC[] THEN DISCH_THEN MATCH_MP_TAC] THEN
+  ASM_REWRITE_TAC[FIELD_INTEGER_MOD_RING; PRIME_P384] THEN
+  ASM_REWRITE_TAC[jacobian_point; INTEGER_MOD_RING_CHAR;
+                  INTEGER_MOD_RING_CLAUSES; IN_INTEGER_MOD_RING_CARRIER] THEN
+  REWRITE_TAC[INT_REM_POS_EQ; INT_LT_REM_EQ; GSYM INT_OF_NUM_CLAUSES] THEN
+  REWRITE_TAC[p_384; b_384] THEN CONV_TAC INT_REDUCE_CONV);;
+
+let represents_p384 = new_definition
+ `represents_p384 P (x,y,z) <=>
+        x < p_384 /\ y < p_384 /\ z < p_384 /\
+        weierstrass_of_jacobian (integer_mod_ring p_384)
+         (tripled (montgomery_decode (384,p_384)) (x,y,z)) = P`;;
+
+let represents2_p384 = new_definition
+ `represents2_p384 P (x,y) <=>
+        x < p_384 /\ y < p_384 /\
+        SOME(paired (montgomery_decode (384,p_384)) (x,y)) = P`;;
+
 let P384_MONTJMIXADD_CORRECT = time prove
  (`!p3 p1 t1 p2 t2 pc stackpointer.
         ALL (nonoverlapping (stackpointer,312))
-            [(word pc,0x3b3a); (p1,144); (p2,96); (p3,144)] /\
-        nonoverlapping (p3,144) (word pc,0x3b3a)
+            [(word pc,0x3c05); (p1,144); (p2,96); (p3,144)] /\
+        nonoverlapping (p3,144) (word pc,0x3c05)
         ==> ensures x86
              (\s. bytes_loaded s (word pc) (BUTLAST p384_montjmixadd_mc) /\
                   read RIP s = word(pc + 0x11) /\
@@ -5225,19 +5345,12 @@ let P384_MONTJMIXADD_CORRECT = time prove
                   C_ARGUMENTS [p3; p1; p2] s /\
                   bignum_triple_from_memory (p1,6) s = t1 /\
                   bignum_pair_from_memory (p2,6) s = t2)
-             (\s. read RIP s = word (pc + 0x3b28) /\
-                  (!x1 y1 z1 x2 y2 z2.
-                        ~(z1 = &0) /\ z2 = &1 /\
-                        ~(jacobian_eq (integer_mod_ring p_384)
-                                      (x1,y1,z1) (x2,y2,z2)) /\
-                        ~(jacobian_eq (integer_mod_ring p_384)
-                                      (jacobian_neg nistp384 (x1,y1,z1))
-                                      (x2,y2,z2)) /\
-                        t1 = tripled nistp384_encode (x1,y1,z1) /\
-                        t2 = paired nistp384_encode (x2,y2)
-                        ==> bignum_triple_from_memory(p3,6) s =
-                            tripled nistp384_encode
-                             (jacobian_add nistp384 (x1,y1,z1) (x2,y2,z2))))
+             (\s. read RIP s = word (pc + 0x3bf3) /\
+                  !P1 P2. represents_p384 P1 t1 /\
+                          represents2_p384 P2 t2 /\
+                          ~(P1 = P2)
+                          ==> represents_p384 (group_mul p384_group P1 P2)
+                               (bignum_triple_from_memory(p3,6) s))
           (MAYCHANGE [RIP; RDI; RSI; RAX; RDX; RCX; R8; R9; R10; R11;
                       RBX; RBP; R12; R13; R14; R15] ,,
            MAYCHANGE SOME_FLAGS ,,
@@ -5273,65 +5386,112 @@ let P384_MONTJMIXADD_CORRECT = time prove
   LOCAL_MONTMUL_P384_TAC 0 ["t2";"yd";"t2"] THEN
   LOCAL_SUB_P384_TAC 1 ["resy";"t2";"t1"] THEN
 
-  BIGNUM_LDIGITIZE_TAC "resx"
+  BIGNUM_LDIGITIZE_TAC "z1_"
+   `read (memory :> bytes (word_add p1 (word 96),8 * 6)) s34` THEN
+  BIGNUM_LDIGITIZE_TAC "x2_"
+   `read (memory :> bytes (p2,8 * 6)) s34` THEN
+  BIGNUM_LDIGITIZE_TAC "y2_"
+   `read (memory :> bytes (word_add p2 (word 48),8 * 6)) s34` THEN
+  BIGNUM_LDIGITIZE_TAC "resx_"
    `read (memory :> bytes (stackpointer,8 * 6)) s34` THEN
-  BIGNUM_LDIGITIZE_TAC "resy"
+  BIGNUM_LDIGITIZE_TAC "resy_"
    `read (memory :> bytes (word_add stackpointer (word 192),8 * 6)) s34` THEN
-  BIGNUM_LDIGITIZE_TAC "resz"
+  BIGNUM_LDIGITIZE_TAC "resz_"
    `read (memory :> bytes (word_add stackpointer (word 240),8 * 6)) s34` THEN
-  X86_STEPS_TAC P384_MONTJMIXADD_EXEC (35--70) THEN
+
+  X86_STEPS_TAC P384_MONTJMIXADD_EXEC (35--114) THEN
   CONV_TAC(ONCE_DEPTH_CONV BIGNUM_LEXPAND_CONV) THEN
   ENSURES_FINAL_STATE_TAC THEN ASM_REWRITE_TAC[] THEN
-  DISCARD_STATE_TAC "s70" THEN
+  DISCARD_STATE_TAC "s114" THEN
   DISCARD_MATCHING_ASSUMPTIONS [`nonoverlapping_modulo a b c`] THEN
+  REWRITE_TAC[WORD_BITWISE_RULE
+    `word_or (word_or (word_or x0 x2) x4)
+             (word_or (word_or x1 x3) x5) =
+     word_or x0 (word_or x1 (word_or x2 (word_or x3 (word_or x4 x5))))`] THEN
 
-  MAP_EVERY X_GEN_TAC
-   [`x1':int`; `y1':int`; `z1':int`; `x2':int`; `y2':int`; `z2':int`] THEN
-  DISCH_THEN(CONJUNCTS_THEN2 ASSUME_TAC MP_TAC) THEN
-  GEN_REWRITE_TAC I [IMP_CONJ] THEN DISCH_THEN SUBST_ALL_TAC THEN
-  REPLICATE_TAC 2 (DISCH_THEN(CONJUNCTS_THEN2 ASSUME_TAC MP_TAC)) THEN
-  REWRITE_TAC[tripled; paired; nistp384_encode; montgomery_encode; PAIR_EQ] THEN
-  DISCH_THEN(REPEAT_TCL CONJUNCTS_THEN
-   (STRIP_ASSUME_TAC o MATCH_MP unilemma2)) THEN
-
+  MAP_EVERY X_GEN_TAC [`P1:(int#int)option`; `P2:(int#int)option`] THEN
+  REWRITE_TAC[represents_p384; represents2_p384; tripled; paired] THEN
+  REWRITE_TAC[montgomery_decode; INT_OF_NUM_CLAUSES; INT_OF_NUM_REM] THEN
+  STRIP_TAC THEN
   REPEAT(FIRST_X_ASSUM(MP_TAC o check (is_imp o concl))) THEN
   REPEAT(ANTS_TAC THENL
    [REWRITE_TAC[p_384] THEN RULE_ASSUM_TAC(REWRITE_RULE[p_384]) THEN
     CONV_TAC NUM_REDUCE_CONV THEN ASM BOUNDER_TAC[];
     (DISCH_THEN(STRIP_ASSUME_TAC o MATCH_MP unilemma0) ORELSE
-     DISCH_THEN(STRIP_ASSUME_TAC o MATCH_MP unilemma1))]) THEN
+     DISCH_THEN(STRIP_ASSUME_TAC o MATCH_MP unilemma1) ORELSE
+     STRIP_TAC)]) THEN
+  REWRITE_TAC[WORD_SUB_0; VAL_EQ_0; INT_OF_NUM_EQ; WORD_OR_EQ_0] THEN
+  REWRITE_TAC[GSYM CONJ_ASSOC] THEN
+  MP_TAC(SPEC `[z1_0:int64;z1_1;z1_2;z1_3;z1_4;z1_5]`
+    BIGNUM_OF_WORDLIST_EQ_0) THEN
+  ASM_REWRITE_TAC[ALL; GSYM INT_OF_NUM_EQ] THEN
+  DISCH_THEN(SUBST1_TAC o SYM) THEN REWRITE_TAC[COND_SWAP] THEN
+  COND_CASES_TAC THEN ASM_REWRITE_TAC[] THENL
+   [REWRITE_TAC[bignum_of_wordlist] THEN
+    CONV_TAC(DEPTH_CONV WORD_NUM_RED_CONV) THEN
+    CONJ_TAC THENL [REWRITE_TAC[p_384] THEN ARITH_TAC; ALL_TAC] THEN
+    REWRITE_TAC[p_384] THEN
+    CONV_TAC(LAND_CONV(funpow 3 RAND_CONV
+     (ONCE_DEPTH_CONV INVERSE_MOD_CONV))) THEN
+    CONV_TAC(ONCE_DEPTH_CONV NUM_MULT_CONV) THEN
+    ONCE_REWRITE_TAC[GSYM MOD_MOD_REFL] THEN
+    CONV_TAC(ONCE_DEPTH_CONV NUM_MOD_CONV) THEN
+    REWRITE_TAC[GSYM p_384; GSYM(NUM_REDUCE_CONV `2 EXP 384`)] THEN
+    REWRITE_TAC[MOD_MOD_REFL] THEN
+    REWRITE_TAC[GSYM INT_OF_NUM_REM; GSYM INT_OF_NUM_CLAUSES] THEN
+    REWRITE_TAC[weierstrass_of_affine_p384] THEN
+    ASM_REWRITE_TAC[INT_OF_NUM_REM; INT_OF_NUM_CLAUSES] THEN
+    EXPAND_TAC "P1" THEN REWRITE_TAC[GSYM INT_OF_NUM_REM] THEN
+    ASM_REWRITE_TAC[GSYM INT_OF_NUM_CLAUSES] THEN
+    REWRITE_TAC[INT_MUL_RZERO; INT_REM_ZERO] THEN
+    REWRITE_TAC[weierstrass_of_jacobian; INTEGER_MOD_RING_CLAUSES] THEN
+    REWRITE_TAC[P384_GROUP; weierstrass_add];
+    ALL_TAC] THEN
+  MAP_EVERY (MP_TAC o C SPEC unreplemma)
+   [`y2:num`; `x2:num`; `z1:num`; `y1:num`; `x1:num`] THEN
+  MAP_EVERY (fun t -> ABBREV_TAC t THEN POP_ASSUM(K ALL_TAC))
+   [`x1d = inverse_mod p_384 (2 EXP 384) * x1`;
+    `y1d = inverse_mod p_384 (2 EXP 384) * y1`;
+    `z1d = inverse_mod p_384 (2 EXP 384) * z1`;
+    `x2d = inverse_mod p_384 (2 EXP 384) * x2`;
+    `y2d = inverse_mod p_384 (2 EXP 384) * y2`] THEN
+  ASM_REWRITE_TAC[] THEN REPEAT DISCH_TAC THEN
   REPEAT(FIRST_X_ASSUM(K ALL_TAC o GEN_REWRITE_RULE I [GSYM NOT_LE])) THEN
-
   RULE_ASSUM_TAC(REWRITE_RULE
    [num_congruent; GSYM INT_OF_NUM_CLAUSES; GSYM INT_OF_NUM_REM]) THEN
   RULE_ASSUM_TAC(REWRITE_RULE[GSYM INT_REM_EQ]) THEN
-  RULE_ASSUM_TAC(ONCE_REWRITE_RULE[GSYM INT_SUB_REM; GSYM INT_ADD_REM]) THEN
+  RULE_ASSUM_TAC(CONV_RULE INT_REM_DOWN_CONV) THEN
   RULE_ASSUM_TAC(REWRITE_RULE[INT_POW_2]) THEN
-  RULE_ASSUM_TAC(GEN_REWRITE_RULE (RAND_CONV o TRY_CONV) [lemont]) THEN
-
-  ASM_REWRITE_TAC[jacobian_add; nistp384] THEN
-  ASM_REWRITE_TAC[GSYM nistp384] THEN
-  REWRITE_TAC[INTEGER_MOD_RING_CLAUSES] THEN
-  CONV_TAC INT_REDUCE_CONV THEN ASM_REWRITE_TAC[] THEN
-  CONV_TAC(TOP_DEPTH_CONV let_CONV) THEN
+  RULE_ASSUM_TAC(ONCE_REWRITE_RULE[GSYM INT_ADD_REM; GSYM INT_SUB_REM]) THEN
+  RULE_ASSUM_TAC(ONCE_REWRITE_RULE[lemont; demont]) THEN
+  ASM_REWRITE_TAC[GSYM INT_OF_NUM_CLAUSES; GSYM INT_OF_NUM_REM] THEN
+  REWRITE_TAC[INT_REM_REM] THEN
+  REWRITE_TAC[pumont; dismont; unmont] THEN
+  FIRST_X_ASSUM(MP_TAC o GEN_REWRITE_RULE LAND_CONV [GSYM
+    weierstrass_of_affine_p384]) THEN
+  FIRST_X_ASSUM(MP_TAC o
+    check(can (term_match [] `weierstrass_of_jacobian f j = p`) o concl)) THEN
+  REWRITE_TAC[IMP_IMP] THEN
+  DISCH_THEN(fun th -> STRIP_ASSUME_TAC th THEN MP_TAC th) THEN
+  MATCH_MP_TAC weierstrass_of_jacobian_p384_add THEN ASM_REWRITE_TAC[] THEN
+  ASM_REWRITE_TAC[jacobian_add_unexceptional; nistp384;
+                  INTEGER_MOD_RING_CLAUSES] THEN
+  SUBGOAL_THEN `~(&z1d rem &p_384 = &0)` (fun th -> REWRITE_TAC[th]) THENL
+   [UNDISCH_TAC `~(&z1:int = &0)` THEN ASM_REWRITE_TAC[CONTRAPOS_THM] THEN
+    REWRITE_TAC[INT_REM_EQ_0] THEN CONV_TAC INTEGER_RULE;
+    ALL_TAC] THEN
+  REWRITE_TAC[p_384] THEN CONV_TAC INT_REDUCE_CONV THEN
+  REWRITE_TAC[GSYM p_384] THEN
+  CONV_TAC(TOP_DEPTH_CONV let_CONV) THEN REWRITE_TAC[PAIR_EQ] THEN
   CONV_TAC INT_REM_DOWN_CONV THEN
-  REWRITE_TAC[tripled; paired; nistp384_encode; montgomery_encode] THEN
-  REWRITE_TAC[PAIR_EQ; GSYM INT_OF_NUM_EQ; nintlemma] THEN
-  CONV_TAC INT_REM_DOWN_CONV THEN
-
-  ASM_REWRITE_TAC[pumont; INT_REM_REM; GSYM INT_ADD_LDISTRIB;
-                GSYM INT_ADD_LDISTRIB; GSYM INT_SUB_LDISTRIB;
-                INT_SUB_REM; INT_ADD_REM] THEN
-
-  REPEAT CONJ_TAC THEN AP_THM_TAC THEN AP_TERM_TAC THEN AP_TERM_TAC THEN
-  INT_ARITH_TAC);;
+  REPEAT CONJ_TAC THEN AP_THM_TAC THEN AP_TERM_TAC THEN INT_ARITH_TAC);;
 
 let P384_MONTJMIXADD_SUBROUTINE_CORRECT = time prove
  (`!p3 p1 t1 p2 t2 pc stackpointer returnaddress.
         ALL (nonoverlapping (word_sub stackpointer (word 360),360))
-            [(word pc,0x3b3a); (p1,144); (p2,96)] /\
+            [(word pc,0x3c05); (p1,144); (p2,96)] /\
         ALL (nonoverlapping (p3,144))
-            [(word pc,0x3b3a); (word_sub stackpointer (word 360),368)]
+            [(word pc,0x3c05); (word_sub stackpointer (word 360),368)]
         ==> ensures x86
              (\s. bytes_loaded s (word pc) p384_montjmixadd_mc /\
                   read RIP s = word pc /\
@@ -5342,18 +5502,11 @@ let P384_MONTJMIXADD_SUBROUTINE_CORRECT = time prove
                   bignum_pair_from_memory (p2,6) s = t2)
              (\s. read RIP s = returnaddress /\
                   read RSP s = word_add stackpointer (word 8) /\
-                  (!x1 y1 z1 x2 y2 z2.
-                        ~(z1 = &0) /\ z2 = &1 /\
-                        ~(jacobian_eq (integer_mod_ring p_384)
-                                      (x1,y1,z1) (x2,y2,z2)) /\
-                        ~(jacobian_eq (integer_mod_ring p_384)
-                                      (jacobian_neg nistp384 (x1,y1,z1))
-                                      (x2,y2,z2)) /\
-                        t1 = tripled nistp384_encode (x1,y1,z1) /\
-                        t2 = paired nistp384_encode (x2,y2)
-                        ==> bignum_triple_from_memory(p3,6) s =
-                            tripled nistp384_encode
-                             (jacobian_add nistp384 (x1,y1,z1) (x2,y2,z2))))
+                  !P1 P2. represents_p384 P1 t1 /\
+                          represents2_p384 P2 t2 /\
+                          ~(P1 = P2)
+                          ==> represents_p384 (group_mul p384_group P1 P2)
+                               (bignum_triple_from_memory(p3,6) s))
           (MAYCHANGE [RSP] ,, MAYCHANGE_REGS_AND_FLAGS_PERMITTED_BY_ABI ,,
            MAYCHANGE [memory :> bytes(p3,144);
                       memory :> bytes(word_sub stackpointer (word 360),360)])`,
@@ -5370,9 +5523,9 @@ let windows_p384_montjmixadd_mc = define_from_elf "windows_p384_montjmixadd_mc"
 let WINDOWS_P384_MONTJMIXADD_SUBROUTINE_CORRECT = time prove
  (`!p3 p1 t1 p2 t2 pc stackpointer returnaddress.
         ALL (nonoverlapping (word_sub stackpointer (word 376),376))
-            [(word pc,0x3b47); (p1,144); (p2,96)] /\
+            [(word pc,0x3c12); (p1,144); (p2,96)] /\
         ALL (nonoverlapping (p3,144))
-            [(word pc,0x3b47); (word_sub stackpointer (word 376),384)]
+            [(word pc,0x3c12); (word_sub stackpointer (word 376),384)]
         ==> ensures x86
              (\s. bytes_loaded s (word pc) windows_p384_montjmixadd_mc /\
                   read RIP s = word pc /\
@@ -5383,18 +5536,11 @@ let WINDOWS_P384_MONTJMIXADD_SUBROUTINE_CORRECT = time prove
                   bignum_pair_from_memory (p2,6) s = t2)
              (\s. read RIP s = returnaddress /\
                   read RSP s = word_add stackpointer (word 8) /\
-                  (!x1 y1 z1 x2 y2 z2.
-                        ~(z1 = &0) /\ z2 = &1 /\
-                        ~(jacobian_eq (integer_mod_ring p_384)
-                                      (x1,y1,z1) (x2,y2,z2)) /\
-                        ~(jacobian_eq (integer_mod_ring p_384)
-                                      (jacobian_neg nistp384 (x1,y1,z1))
-                                      (x2,y2,z2)) /\
-                        t1 = tripled nistp384_encode (x1,y1,z1) /\
-                        t2 = paired nistp384_encode (x2,y2)
-                        ==> bignum_triple_from_memory(p3,6) s =
-                            tripled nistp384_encode
-                             (jacobian_add nistp384 (x1,y1,z1) (x2,y2,z2))))
+                  !P1 P2. represents_p384 P1 t1 /\
+                          represents2_p384 P2 t2 /\
+                          ~(P1 = P2)
+                          ==> represents_p384 (group_mul p384_group P1 P2)
+                               (bignum_triple_from_memory(p3,6) s))
           (MAYCHANGE [RSP] ,, WINDOWS_MAYCHANGE_REGS_AND_FLAGS_PERMITTED_BY_ABI ,,
            MAYCHANGE [memory :> bytes(p3,144);
                       memory :> bytes(word_sub stackpointer (word 376),376)])`,
