arm/proofs/secp256k1_jmixadd.ml
@@ -1179,18 +1179,41 @@ let secp256k1_jmixadd_mc = define_assert_from_elf
   0xda1f0108;       (* arm_SBC X8 X8 XZR *)
   0xa9081be5;       (* arm_STP X5 X6 SP (Immediate_Offset (iword (&128))) *)
   0xa90923e7;       (* arm_STP X7 X8 SP (Immediate_Offset (iword (&144))) *)
+  0xa9440600;       (* arm_LDP X0 X1 X16 (Immediate_Offset (iword (&64))) *)
+  0xa9450e02;       (* arm_LDP X2 X3 X16 (Immediate_Offset (iword (&80))) *)
+  0xaa010004;       (* arm_ORR X4 X0 X1 *)
+  0xaa030045;       (* arm_ORR X5 X2 X3 *)
+  0xaa050084;       (* arm_ORR X4 X4 X5 *)
+  0xeb1f009f;       (* arm_CMP X4 XZR *)
   0xa94007e0;       (* arm_LDP X0 X1 SP (Immediate_Offset (iword (&0))) *)
+  0xa940362c;       (* arm_LDP X12 X13 X17 (Immediate_Offset (iword (&0))) *)
+  0x9a8c1000;       (* arm_CSEL X0 X0 X12 Condition_NE *)
+  0x9a8d1021;       (* arm_CSEL X1 X1 X13 Condition_NE *)
   0xa9410fe2;       (* arm_LDP X2 X3 SP (Immediate_Offset (iword (&16))) *)
+  0xa941362c;       (* arm_LDP X12 X13 X17 (Immediate_Offset (iword (&16))) *)
+  0x9a8c1042;       (* arm_CSEL X2 X2 X12 Condition_NE *)
+  0x9a8d1063;       (* arm_CSEL X3 X3 X13 Condition_NE *)
+  0xa94817e4;       (* arm_LDP X4 X5 SP (Immediate_Offset (iword (&128))) *)
+  0xa942362c;       (* arm_LDP X12 X13 X17 (Immediate_Offset (iword (&32))) *)
+  0x9a8c1084;       (* arm_CSEL X4 X4 X12 Condition_NE *)
+  0x9a8d10a5;       (* arm_CSEL X5 X5 X13 Condition_NE *)
+  0xa9491fe6;       (* arm_LDP X6 X7 SP (Immediate_Offset (iword (&144))) *)
+  0xa943362c;       (* arm_LDP X12 X13 X17 (Immediate_Offset (iword (&48))) *)
+  0x9a8c10c6;       (* arm_CSEL X6 X6 X12 Condition_NE *)
+  0x9a8d10e7;       (* arm_CSEL X7 X7 X13 Condition_NE *)
+  0xa94a27e8;       (* arm_LDP X8 X9 SP (Immediate_Offset (iword (&160))) *)
+  0xd280002c;       (* arm_MOV X12 (rvalue (word 1)) *)
+  0x9a8c1108;       (* arm_CSEL X8 X8 X12 Condition_NE *)
+  0x9a9f1129;       (* arm_CSEL X9 X9 XZR Condition_NE *)
+  0xa94b2fea;       (* arm_LDP X10 X11 SP (Immediate_Offset (iword (&176))) *)
+  0x9a9f114a;       (* arm_CSEL X10 X10 XZR Condition_NE *)
+  0x9a9f116b;       (* arm_CSEL X11 X11 XZR Condition_NE *)
   0xa90005e0;       (* arm_STP X0 X1 X15 (Immediate_Offset (iword (&0))) *)
   0xa9010de2;       (* arm_STP X2 X3 X15 (Immediate_Offset (iword (&16))) *)
-  0xa94807e0;       (* arm_LDP X0 X1 SP (Immediate_Offset (iword (&128))) *)
-  0xa9490fe2;       (* arm_LDP X2 X3 SP (Immediate_Offset (iword (&144))) *)
-  0xa90205e0;       (* arm_STP X0 X1 X15 (Immediate_Offset (iword (&32))) *)
-  0xa9030de2;       (* arm_STP X2 X3 X15 (Immediate_Offset (iword (&48))) *)
-  0xa94a07e0;       (* arm_LDP X0 X1 SP (Immediate_Offset (iword (&160))) *)
-  0xa94b0fe2;       (* arm_LDP X2 X3 SP (Immediate_Offset (iword (&176))) *)
-  0xa90405e0;       (* arm_STP X0 X1 X15 (Immediate_Offset (iword (&64))) *)
-  0xa9050de2;       (* arm_STP X2 X3 X15 (Immediate_Offset (iword (&80))) *)
+  0xa90215e4;       (* arm_STP X4 X5 X15 (Immediate_Offset (iword (&32))) *)
+  0xa9031de6;       (* arm_STP X6 X7 X15 (Immediate_Offset (iword (&48))) *)
+  0xa90425e8;       (* arm_STP X8 X9 X15 (Immediate_Offset (iword (&64))) *)
+  0xa9052dea;       (* arm_STP X10 X11 X15 (Immediate_Offset (iword (&80))) *)
   0x910303ff;       (* arm_ADD SP SP (rvalue (word 192)) *)
   0xd65f03c0        (* arm_RET X30 *)
 ];;
@@ -1244,7 +1267,7 @@ let LOCAL_SQR_P256K1_TAC =
     !n. read(memory :> bytes(word_add (read p1 t) (word n1),8 * 4)) t = n
     ==>
     aligned 16 (read SP t) /\
-    nonoverlapping (word pc,0x124c) (word_add (read p3 t) (word n3),32)
+    nonoverlapping (word pc,0x12a8) (word_add (read p3 t) (word n3),32)
     ==> ensures arm
          (\s. aligned_bytes_loaded s (word pc) secp256k1_jmixadd_mc /\
               read PC s = pcin /\
@@ -1381,7 +1404,7 @@ let LOCAL_MUL_P256K1_TAC =
     !n. read(memory :> bytes(word_add (read p2 t) (word n2),8 * 4)) t = n
     ==>
     aligned 16 (read SP t) /\
-    nonoverlapping (word pc,0x124c) (word_add (read p3 t) (word n3),32)
+    nonoverlapping (word pc,0x12a8) (word_add (read p3 t) (word n3),32)
     ==> ensures arm
          (\s. aligned_bytes_loaded s (word pc) secp256k1_jmixadd_mc /\
               read PC s = pcin /\
@@ -1520,7 +1543,7 @@ let LOCAL_SUB_P256K1_TAC =
     !n. read(memory :> bytes(word_add (read p2 t) (word n2),8 * 4)) t = n
     ==>
     aligned 16 (read SP t) /\
-    nonoverlapping (word pc,0x124c) (word_add (read p3 t) (word n3),32)
+    nonoverlapping (word pc,0x12a8) (word_add (read p3 t) (word n3),32)
     ==> ensures arm
          (\s. aligned_bytes_loaded s (word pc) secp256k1_jmixadd_mc /\
               read PC s = pcin /\
@@ -1668,8 +1691,8 @@ let SECP256K1_JMIXADD_CORRECT = time prove
  (`!p3 p1 t1 p2 t2 pc stackpointer.
         aligned 16 stackpointer /\
         ALL (nonoverlapping (stackpointer,192))
-            [(word pc,0x124c); (p1,96); (p2,64); (p3,96)] /\
-        nonoverlapping (p3,96) (word pc,0x124c)
+            [(word pc,0x12a8); (p1,96); (p2,64); (p3,96)] /\
+        nonoverlapping (p3,96) (word pc,0x12a8)
         ==> ensures arm
              (\s. aligned_bytes_loaded s (word pc) secp256k1_jmixadd_mc /\
                   read PC s = word(pc + 0x4) /\
@@ -1677,11 +1700,11 @@ let SECP256K1_JMIXADD_CORRECT = time prove
                   C_ARGUMENTS [p3; p1; p2] s /\
                   bignum_triple_from_memory (p1,4) s = t1 /\
                   bignum_pair_from_memory (p2,4) s = t2)
-             (\s. read PC s = word (pc + 0x1244) /\
+             (\s. read PC s = word (pc + 0x12a0) /\
                  !P1 P2. represents_p256k1 P1 t1 /\
-                          represents2_p256k1 P2 t2 /\
-                          ~(P1 = NONE) /\ ~(P1 = P2)
-                          ==> represents_p256k1(group_mul p256k1_group P1 P2)
+                         represents2_p256k1 P2 t2 /\
+                         ~(P1 = P2)
+                         ==> represents_p256k1(group_mul p256k1_group P1 P2)
                                (bignum_triple_from_memory(p3,4) s))
           (MAYCHANGE [PC; X0; X1; X2; X3; X4; X5; X6; X7; X8; X9; X10;
                       X11; X12; X13; X14; X15; X16; X17] ,,
@@ -1718,16 +1741,24 @@ let SECP256K1_JMIXADD_CORRECT = time prove
   LOCAL_MUL_P256K1_TAC 0 ["t2";"yd";"t2"] THEN
   LOCAL_SUB_P256K1_TAC 0 ["resy";"t2";"t1"] THEN
 
-  BIGNUM_LDIGITIZE_TAC "resx"
+
+  BIGNUM_LDIGITIZE_TAC "z1_"
+   `read (memory :> bytes (word_add p1 (word 64),8 * 4)) s21` THEN
+  BIGNUM_LDIGITIZE_TAC "x2_"
+   `read (memory :> bytes (p2,8 * 4)) s21` THEN
+  BIGNUM_LDIGITIZE_TAC "y2_"
+   `read (memory :> bytes (word_add p2 (word 32),8 * 4)) s21` THEN
+  BIGNUM_LDIGITIZE_TAC "resx_"
    `read (memory :> bytes (stackpointer,8 * 4)) s21` THEN
-  BIGNUM_LDIGITIZE_TAC "resy"
+  BIGNUM_LDIGITIZE_TAC "resy_"
    `read (memory :> bytes (word_add stackpointer (word 128),8 * 4)) s21` THEN
-  BIGNUM_LDIGITIZE_TAC "resz"
+  BIGNUM_LDIGITIZE_TAC "resz_"
    `read (memory :> bytes (word_add stackpointer (word 160),8 * 4)) s21` THEN
-  ARM_STEPS_TAC SECP256K1_JMIXADD_EXEC (22--33) THEN
+
+  ARM_STEPS_TAC SECP256K1_JMIXADD_EXEC (22--56) THEN
   CONV_TAC(ONCE_DEPTH_CONV BIGNUM_LEXPAND_CONV) THEN
   ENSURES_FINAL_STATE_TAC THEN ASM_REWRITE_TAC[] THEN
-  DISCARD_STATE_TAC "s33" THEN
+  DISCARD_STATE_TAC "s56" THEN
   DISCARD_MATCHING_ASSUMPTIONS [`nonoverlapping_modulo a b c`] THEN
 
   MAP_EVERY X_GEN_TAC [`P1:(int#int)option`; `P2:(int#int)option`] THEN
@@ -1741,6 +1772,26 @@ let SECP256K1_JMIXADD_CORRECT = time prove
     (DISCH_THEN(STRIP_ASSUME_TAC o MATCH_MP unilemma0) ORELSE
      DISCH_THEN(STRIP_ASSUME_TAC o MATCH_MP unilemma1) ORELSE
      STRIP_TAC)]) THEN
+  REWRITE_TAC[WORD_SUB_0; VAL_EQ_0; INT_OF_NUM_EQ; WORD_OR_EQ_0] THEN
+  REWRITE_TAC[GSYM CONJ_ASSOC] THEN
+  MP_TAC(SPEC `[z1_0:int64;z1_1;z1_2;z1_3]` BIGNUM_OF_WORDLIST_EQ_0) THEN
+  ASM_REWRITE_TAC[ALL; GSYM INT_OF_NUM_EQ] THEN
+  DISCH_THEN(SUBST1_TAC o SYM) THEN REWRITE_TAC[COND_SWAP] THEN
+  COND_CASES_TAC THEN ASM_REWRITE_TAC[] THENL
+   [REWRITE_TAC[bignum_of_wordlist] THEN
+    CONV_TAC(DEPTH_CONV WORD_NUM_RED_CONV) THEN
+    CONJ_TAC THENL [REWRITE_TAC[p_256k1] THEN ARITH_TAC; ALL_TAC] THEN
+    REWRITE_TAC[GSYM INT_OF_NUM_REM; GSYM INT_OF_NUM_CLAUSES] THEN
+    REWRITE_TAC[weierstrass_of_affine_p256k1] THEN
+    ASM_REWRITE_TAC[INT_OF_NUM_REM; INT_OF_NUM_CLAUSES] THEN
+    EXPAND_TAC "P1" THEN REWRITE_TAC[GSYM INT_OF_NUM_REM] THEN
+    ASM_REWRITE_TAC[GSYM INT_OF_NUM_CLAUSES] THEN
+    REWRITE_TAC[INT_MUL_RZERO; INT_REM_ZERO] THEN
+    REWRITE_TAC[weierstrass_of_jacobian; INTEGER_MOD_RING_CLAUSES] THEN
+    REWRITE_TAC[P256K1_GROUP; weierstrass_add];
+    ALL_TAC] THEN
+  SUBGOAL_THEN `~(&z1 rem &p_256k1 = &0)` ASSUME_TAC THENL
+   [ASM_SIMP_TAC[INT_OF_NUM_REM; MOD_LT]; ALL_TAC] THEN
   ASM_REWRITE_TAC[] THEN
   REPEAT(CONJ_TAC THENL [REWRITE_TAC[p_256k1] THEN ARITH_TAC; ALL_TAC]) THEN
   REPEAT(FIRST_X_ASSUM(K ALL_TAC o GEN_REWRITE_RULE I [GSYM NOT_LE])) THEN
@@ -1755,9 +1806,6 @@ let SECP256K1_JMIXADD_CORRECT = time prove
   FIRST_X_ASSUM(MP_TAC o
     check(can (term_match [] `weierstrass_of_jacobian f j = p`) o concl)) THEN
   REWRITE_TAC[IMP_IMP] THEN
-  ASM_CASES_TAC `&z1 rem &p_256k1 = &0` THENL
-   [ASM_REWRITE_TAC[weierstrass_of_jacobian; INTEGER_MOD_RING_CLAUSES];
-    ALL_TAC] THEN
   ASM_REWRITE_TAC[GSYM INT_OF_NUM_REM; GSYM INT_OF_NUM_CLAUSES] THEN
   CONV_TAC INT_REM_DOWN_CONV THEN
   DISCH_THEN(fun th -> STRIP_ASSUME_TAC th THEN MP_TAC th) THEN
@@ -1774,8 +1822,8 @@ let SECP256K1_JMIXADD_SUBROUTINE_CORRECT = time prove
  (`!p3 p1 t1 p2 t2 pc stackpointer returnaddress.
         aligned 16 stackpointer /\
         ALL (nonoverlapping (word_sub stackpointer (word 192),192))
-            [(word pc,0x124c); (p1,96); (p2,64); (p3,96)] /\
-        nonoverlapping (p3,96) (word pc,0x124c)
+            [(word pc,0x12a8); (p1,96); (p2,64); (p3,96)] /\
+        nonoverlapping (p3,96) (word pc,0x12a8)
         ==> ensures arm
              (\s. aligned_bytes_loaded s (word pc) secp256k1_jmixadd_mc /\
                   read PC s = word pc /\
@@ -1786,9 +1834,9 @@ let SECP256K1_JMIXADD_SUBROUTINE_CORRECT = time prove
                   bignum_pair_from_memory (p2,4) s = t2)
              (\s. read PC s = returnaddress /\
                  !P1 P2. represents_p256k1 P1 t1 /\
-                          represents2_p256k1 P2 t2 /\
-                          ~(P1 = NONE) /\ ~(P1 = P2)
-                          ==> represents_p256k1(group_mul p256k1_group P1 P2)
+                         represents2_p256k1 P2 t2 /\
+                         ~(P1 = P2)
+                         ==> represents_p256k1(group_mul p256k1_group P1 P2)
                                (bignum_triple_from_memory(p3,4) s))
           (MAYCHANGE_REGS_AND_FLAGS_PERMITTED_BY_ABI ,,
            MAYCHANGE [memory :> bytes(p3,96);
